work in progress

src/axiomatic/Gevents.v
@@ -15,8 +15,7 @@ Definition thread_id := IdentMap.key.
 Inductive label := 
   | Aload (l:Loc.t) (v:Const.t) (o:Ordering.t)
   | Astore (l:Loc.t) (v:Const.t) (o:Ordering.t)
-  | Arfence (o:Ordering.t)
-  | Awfence (o:Ordering.t).
+  | Afence (or ow:Ordering.t).
 
 Inductive event := 
   | Event (id: act_id) (tid: thread_id) (lb:label).
@@ -37,54 +36,64 @@ Definition lab a :=
   end.
 
 Definition loc a :=
-  match (lab a) with
+  match lab a with
   | Aload l _ _
   | Astore l _ _ => Some l
   | _ => None
   end.
 
 Definition val a :=
-  match (lab a) with
+  match lab a with
   | Aload  _ v _
   | Astore _ v _ => Some v
   | _ => None
   end.
 
-Definition ord a :=
-  match (lab a) with
-  | Aload  _ _ o
-  | Astore _ _ o
-  | Arfence o 
-  | Awfence o => o
-  end.
-
 Definition is_read a := 
-  match (lab a) with
+  match lab a with
   | Aload  _ _ _ => True
   | _ => False
   end.
 
 Definition is_write a := 
-  match (lab a) with
+  match lab a with
   | Astore _ _ _ => True
   | _ => False
   end.
 
-Definition is_rfence a := 
-  match (lab a) with
-  | Arfence _ => True
+Definition is_fence a := 
+  match lab a with
+  | Afence _ _ => True
   | _ => False
   end.
 
-Definition is_wfence a := 
-  match (lab a) with
-  | Awfence  _ => True
-  | _ => False
+Definition is_rlx_rw a : Prop :=
+  match lab a with
+    | Aload  _ _ o
+    | Astore  _ _ o => Ordering.le Ordering.relaxed o
+    | _ => False
   end.
 
-Definition is_rlx a :Prop := Ordering.le Ordering.relaxed (ord a).
-Definition is_ra  a :Prop := Ordering.le Ordering.acqrel  (ord a).
-Definition is_sc  a :Prop := Ordering.le Ordering.seqcst  (ord a).
+Definition is_acq a : Prop :=
+  match lab a with
+    | Aload  _ _ o
+    | Afence o _ => Ordering.le Ordering.acqrel o
+    | _ => False
+  end.
+
+Definition is_rel a : Prop :=
+  match lab a with
+    | Astore  _ _ o
+    | Afence _ o => Ordering.le Ordering.acqrel o
+    | _ => False
+  end.
+
+Definition is_sc a : Prop :=
+  match lab a with
+    | Astore  _ _ o
+    | Aload  _ _ o
+    | Afence _ o => Ordering.le Ordering.seqcst o
+  end.
 
 (** * Basic Lemmas *)
 
@@ -92,45 +101,45 @@ Lemma read_non_write a (A: is_read a) : ~ is_write a.
 Proof. destruct a; destruct lb; ins. Qed.
 Lemma write_non_read a (A: is_write a) : ~ is_read a.
 Proof. destruct a; destruct lb; ins. Qed.
-Lemma wfence_non_read a (A: is_wfence a) : ~ is_read a.
+Lemma fence_non_read a (A: is_fence a) : ~ is_read a.
 Proof. destruct a; destruct lb; ins. Qed.
-Lemma write_non_rfence a (A: is_write a) : ~ is_rfence a.
-Proof. destruct a; destruct lb; ins. Qed.
-Lemma write_non_wfence a (A: is_write a) : ~ is_wfence a.
+Lemma write_non_fence a (A: is_write a) : ~ is_fence a.
 Proof. destruct a; destruct lb; ins. Qed.
 
 
 Lemma write_has_location a (WRITE: is_write a) : exists l, loc a = Some l.
 Proof. unfold loc; destruct a; destruct lb; ins; eauto. Qed.
+(*
 Lemma ra_is_rlx a (RA: is_ra a) : is_rlx a.
 Proof. destruct a; destruct lb; destruct o; ins. Qed.
 Lemma sc_is_rlx a (SC: is_sc a) : is_rlx a.
 Proof. destruct a; destruct lb; destruct o; ins. Qed.
 Lemma sc_is_ra a (SC: is_sc a) : is_ra a.
 Proof. destruct a; destruct lb; destruct o; ins. Qed.
+*)
 
 Lemma read_is_read a l v o (A: lab a = Aload l v o) : is_read a.
 Proof. destruct a; destruct lb; ins. Qed.
 Lemma write_is_write a l v o (A: lab a = Astore l v o) : is_write a.
 Proof. destruct a; destruct lb; ins. Qed.
 
-Lemma read_rlx a l v o (A: lab a = Aload l v o) : Ordering.le Ordering.relaxed o -> is_rlx a.
-Proof. unfold is_rlx; unfold ord; rewrite A; done. Qed.
-Lemma read_ra a l v o (A: lab a = Aload l v o) : Ordering.le Ordering.acqrel o -> is_ra a.
-Proof. unfold is_ra; unfold ord; rewrite A; done. Qed.
+Lemma read_rlx a l v o (A: lab a = Aload l v o) : Ordering.le Ordering.relaxed o -> is_rlx_rw a.
+Proof. destruct a; ins; rewrite A; done. Qed.
+Lemma read_acq a l v o (A: lab a = Aload l v o) : Ordering.le Ordering.acqrel o -> is_acq a.
+Proof. destruct a; ins; rewrite A; done. Qed.
 Lemma read_sc a l v o (A: lab a = Aload l v o) : Ordering.le Ordering.seqcst o -> is_sc a.
-Proof. unfold is_sc; unfold ord; rewrite A; done. Qed.
+Proof. destruct a; ins; rewrite A; done. Qed.
 
-Lemma write_rlx a l v o (A: lab a = Astore l v o) : Ordering.le Ordering.relaxed o -> is_rlx a.
-Proof. unfold is_rlx; unfold ord; rewrite A; done. Qed.
-Lemma write_ra a l v o (A: lab a = Astore l v o) : Ordering.le Ordering.acqrel o -> is_ra a.
-Proof. unfold is_ra; unfold ord; rewrite A; done. Qed.
+Lemma write_rlx a l v o (A: lab a = Astore l v o) : Ordering.le Ordering.relaxed o -> is_rlx_rw a.
+Proof. destruct a; ins; rewrite A; done. Qed.
+Lemma write_rel a l v o (A: lab a = Astore l v o) : Ordering.le Ordering.acqrel o -> is_rel a.
+Proof. destruct a; ins; rewrite A; done. Qed.
 Lemma write_sc a l v o (A: lab a = Astore l v o) : Ordering.le Ordering.seqcst o -> is_sc a.
-Proof. unfold is_sc; unfold ord; rewrite A; done. Qed.
+Proof. destruct a; ins; rewrite A; done. Qed.
 
 
-Hint Resolve  read_non_write write_non_read wfence_non_read ra_is_rlx 
-sc_is_rlx sc_is_ra read_is_read read_rlx read_ra read_sc
-write_is_write write_rlx write_ra write_sc 
-write_non_rfence write_non_wfence : acts.
+Hint Resolve  read_non_write write_non_read fence_non_read 
+     read_is_read read_rlx read_acq read_sc
+     write_is_write write_rlx write_rel write_sc 
+     write_non_fence write_non_fence : acts.
 
